Fleshing out stamp representation
Expanding the stamp representation to handle more stamp types.

Stamp.thy
@@ -1,54 +1,178 @@
 theory Stamp
-imports "HOL-Word.Word"
-begin
+  imports 
+    "HOL-Word.Word"
+    "HOL-Library.Float"
+begin            
 
 fun bit_bounds :: "nat \<Rightarrow> (int \<times> int)" where
   "bit_bounds bits = (((2 ^ bits) div 2) * -1, ((2 ^ bits) div 2) - 1)"
 
+definition pos_infinity :: "float" where
+  "pos_infinity = float_of (0 * 2 powr 255)"
+
+definition neg_infinity :: "float" where
+  "neg_infinity = -pos_infinity"
+
 datatype Stamp = 
-  FloatStamp
+  VoidStamp
+  | IntegerStamp (stp_bits: nat) (stpi_lower: int) (stpi_upper: int)
+  | FloatStamp (stp_bits: nat) (stpf_lower: float) (stpf_upper: float)
+  | KlassPointerStamp (stp_nonNull: bool) (stp_alwaysNull: bool)
+  | MethodCountersPointerStamp (stp_nonNull: bool) (stp_alwaysNull: bool)
+  | MethodPointersStamp (stp_nonNull: bool) (stp_alwaysNull: bool)
+  | ObjectStamp (stp_type: string) (stp_exactType: bool) (stp_nonNull: bool) (stp_alwaysNull: bool)
+  | RawPointerStamp (stp_nonNull: bool) (stp_alwaysNull: bool)
   | IllegalStamp
-  | IntegerStamp (stp_bits: nat) (stp_lower: int) (stp_upper: int)
-  | KlassPointerStamp
-  | MethodCountersPointerStamp
-  | MethodPointersStamp
-  | ObjectStamp
-  | RawPointerStamp
-  | VoidStamp
-
-
-fun meet :: "Stamp \<Rightarrow> Stamp \<Rightarrow> Stamp" where
-  "meet (IntegerStamp b1 l1 u1) (IntegerStamp b2 l2 u2) = (
-    if b1 \<noteq> b2 then IllegalStamp else 
-    (IntegerStamp b1 (min l1 l2) (max u1 u2))
-  )" | 
-  "meet s1 s2 = IllegalStamp"
-
-fun join :: "Stamp \<Rightarrow> Stamp \<Rightarrow> Stamp" where
-  "join (IntegerStamp b1 l1 u1) (IntegerStamp b2 l2 u2) = (
-    if b1 \<noteq> b2 then IllegalStamp else 
-    (IntegerStamp b1 (max l1 l2) (min u1 u2))
-  )" | 
-  "join s1 s2 = IllegalStamp"
 
 fun unrestricted :: "Stamp \<Rightarrow> Stamp" where
+  "unrestricted VoidStamp = VoidStamp" |
   "unrestricted (IntegerStamp bits lower upper) = (IntegerStamp bits (fst (bit_bounds bits)) (snd (bit_bounds bits)))" | 
+  "unrestricted (FloatStamp bits lower upper) = (FloatStamp bits neg_infinity pos_infinity)" | 
+  "unrestricted (KlassPointerStamp nonNull alwaysNull) = (KlassPointerStamp False False)" |
+  "unrestricted (MethodCountersPointerStamp nonNull alwaysNull) = (MethodCountersPointerStamp False False)" |
+  "unrestricted (MethodPointersStamp nonNull alwaysNull) = (MethodPointersStamp False False)" |
+  "unrestricted (ObjectStamp type exactType nonNull alwaysNull) = (ObjectStamp '''' False False False)" |
   "unrestricted _ = IllegalStamp"
 
 fun empty :: "Stamp \<Rightarrow> Stamp" where
+  "empty VoidStamp = VoidStamp" |
   "empty (IntegerStamp bits lower upper) = (IntegerStamp bits (snd (bit_bounds bits)) (fst (bit_bounds bits)))" |
+  "empty (FloatStamp bits lower upper) = (FloatStamp bits pos_infinity neg_infinity)" |
+  "empty (KlassPointerStamp nonNull alwaysNull) = (KlassPointerStamp nonNull alwaysNull)" |
+  "empty (MethodCountersPointerStamp nonNull alwaysNull) = (MethodCountersPointerStamp nonNull alwaysNull)" |
+  "empty (MethodPointersStamp nonNull alwaysNull) = (MethodPointersStamp nonNull alwaysNull)" |
+  "empty (ObjectStamp type exactType nonNull alwaysNull) = (ObjectStamp '''' True True False)" |
   "empty stamp = IllegalStamp"
 
+fun meet :: "Stamp \<Rightarrow> Stamp \<Rightarrow> Stamp" where
+  "meet VoidStamp VoidStamp = VoidStamp" |
+  "meet (IntegerStamp b1 l1 u1) (IntegerStamp b2 l2 u2) = (
+    if b1 \<noteq> b2 then IllegalStamp else 
+    (IntegerStamp b1 (min l1 l2) (max u1 u2))
+  )" |
+  "meet (FloatStamp b1 l1 u1) (FloatStamp b2 l2 u2) = (
+    if b1 \<noteq> b2 then IllegalStamp else 
+    (FloatStamp b1 (min l1 l2) (max u1 u2))
+  )" |
+  "meet (KlassPointerStamp nn1 an1) (KlassPointerStamp nn2 an2) = (
+    KlassPointerStamp (nn1 \<and> nn2) (an1 \<and> an2)
+  )" |
+  "meet (MethodCountersPointerStamp nn1 an1) (MethodCountersPointerStamp nn2 an2) = (
+    MethodCountersPointerStamp (nn1 \<and> nn2) (an1 \<and> an2)
+  )" |
+  "meet (MethodPointersStamp nn1 an1) (MethodPointersStamp nn2 an2) = (
+    MethodPointersStamp (nn1 \<and> nn2) (an1 \<and> an2)
+  )" |
+  "meet s1 s2 = IllegalStamp"
 
-value "unrestricted (IntegerStamp 8 0 10)"
-value "unrestricted (IntegerStamp 16 0 10)"
-value "unrestricted (IntegerStamp 32 0 10)"
+fun join :: "Stamp \<Rightarrow> Stamp \<Rightarrow> Stamp" where
+  "join VoidStamp VoidStamp = VoidStamp" |
+  "join (IntegerStamp b1 l1 u1) (IntegerStamp b2 l2 u2) = (
+    if b1 \<noteq> b2 then IllegalStamp else 
+    (IntegerStamp b1 (max l1 l2) (min u1 u2))
+  )" |
+  "join (FloatStamp b1 l1 u1) (FloatStamp b2 l2 u2) = (
+    if b1 \<noteq> b2 then IllegalStamp else 
+    (FloatStamp b1 (max l1 l2) (min u1 u2))
+  )" |
+  "join (KlassPointerStamp nn1 an1) (KlassPointerStamp nn2 an2) = (
+    if ((nn1 \<or> nn2) \<and> (an1 \<or> an2)) 
+    then (empty (KlassPointerStamp nn1 an1))
+    else (KlassPointerStamp (nn1 \<or> nn2) (an1 \<or> an2))
+  )" |
+  "join (MethodCountersPointerStamp nn1 an1) (MethodCountersPointerStamp nn2 an2) = (
+    if ((nn1 \<or> nn2) \<and> (an1 \<or> an2)) 
+    then (empty (MethodCountersPointerStamp nn1 an1))
+    else (MethodCountersPointerStamp (nn1 \<or> nn2) (an1 \<or> an2))
+  )" |
+  "join (MethodPointersStamp nn1 an1) (MethodPointersStamp nn2 an2) = (
+    if ((nn1 \<or> nn2) \<and> (an1 \<or> an2)) 
+    then (empty (MethodPointersStamp nn1 an1))
+    else (MethodPointersStamp (nn1 \<or> nn2) (an1 \<or> an2))
+  )" |
+  "join s1 s2 = IllegalStamp"
 
-value "empty (IntegerStamp 8 0 10)"
-value "empty (IntegerStamp 16 0 10)"
-value "empty (IntegerStamp 32 0 10)"
 
-value "join (IntegerStamp 32 0 20) (IntegerStamp 32 (-100) 10)"
-value "meet (IntegerStamp 32 0 20) (IntegerStamp 32 (-100) 10)"
+(* Theories/Lemmas *)
+lemma intstamp_bits_eq_meet:
+  assumes "(meet (IntegerStamp b1 l1 u1) (IntegerStamp b2 l2 u2)) = (IntegerStamp b3 l3 u3)"
+  shows "b1 = b3 \<and> b2 = b3"
+  by (metis Stamp.distinct(29) assms meet.simps(2))
+
+lemma intstamp_bits_eq_join:
+  assumes "(join (IntegerStamp b1 l1 u1) (IntegerStamp b2 l2 u2)) = (IntegerStamp b3 l3 u3)"
+  shows "b1 = b3 \<and> b2 = b3"
+  by (metis Stamp.distinct(29) assms join.simps(2))
+
+lemma intstamp_bites_eq_unrestricted:
+  assumes "(unrestricted (IntegerStamp b1 l1 u1)) = (IntegerStamp b2 l2 u2)"
+  shows "b1 = b2"
+  using assms by auto
+
+lemma intstamp_bits_eq_empty:
+  assumes "(empty (IntegerStamp b1 l1 u1)) = (IntegerStamp b2 l2 u2)"
+  shows "b1 = b2"
+  using assms by auto
+
+lemma floatstamp_bits_eq_meet:
+  assumes "(meet (FloatStamp b1 l1 u1) (FloatStamp b2 l2 u2)) = (FloatStamp b3 l3 u3)"
+  shows "b1 = b3 \<and> b2 = b3"
+  by (metis Stamp.distinct(42) assms meet.simps(3))
+
+lemma floatstamp_bits_eq_join:
+  assumes "(join (FloatStamp b1 l1 u1) (FloatStamp b2 l2 u2)) = (FloatStamp b3 l3 u3)"
+  shows "b1 = b3 \<and> b2 = b3"
+  by (metis Stamp.distinct(42) assms join.simps(3))
+
+lemma floatstamp_bites_eq_unrestricted:
+  assumes "(unrestricted (FloatStamp b1 l1 u1)) = (FloatStamp b2 l2 u2)"
+  shows "b1 = b2"
+  using assms by auto
+
+lemma floatstamp_bits_eq_empty:
+  assumes "(empty (FloatStamp b1 l1 u1)) = (FloatStamp b2 l2 u2)"
+  shows "b1 = b2"
+  using assms by auto
+
+(* Manual sanity checks *)
+notepad
+begin
+  have "unrestricted (IntegerStamp 8 0 10) = (IntegerStamp 8 (- 128) 127)"
+    by auto
+  have "unrestricted (IntegerStamp 16 0 10) = (IntegerStamp 16 (- 32768) 32767)"
+    by auto
+  have "unrestricted (IntegerStamp 32 0 10) = (IntegerStamp 32 (- 2147483648) 2147483647)"
+    by auto
+  have "empty (IntegerStamp 8 0 10) = (IntegerStamp 8 127 (- 128))"
+    by auto
+  have "empty (IntegerStamp 16 0 10) = (IntegerStamp 16 32767 (- 32768))"
+    by auto
+  have "empty (IntegerStamp 32 0 10) = (IntegerStamp 32 2147483647 (- 2147483648))"
+    by auto
+  have "join (IntegerStamp 32 0 20) (IntegerStamp 32 (-100) 10) = (IntegerStamp 32 0 10)"
+    by auto
+  have "meet (IntegerStamp 32 0 20) (IntegerStamp 32 (-100) 10) = (IntegerStamp 32 (- 100) 20)"
+    by auto
+end
+
+notepad
+begin
+  have "unrestricted (FloatStamp 8 0 10) = (FloatStamp 8 neg_infinity pos_infinity)"
+    by auto
+  have "unrestricted (FloatStamp 16 0 10) = (FloatStamp 16 neg_infinity pos_infinity)"
+    by auto
+  have "unrestricted (FloatStamp 32 0 10) = (FloatStamp 32 neg_infinity pos_infinity)"
+    by auto
+  have "empty (FloatStamp 8 0 10) = (FloatStamp 8 pos_infinity neg_infinity)"
+    by auto
+  have "empty (FloatStamp 16 0 10) = (FloatStamp 16 pos_infinity neg_infinity)"
+    by auto
+  have "empty (FloatStamp 32 0 10) = (FloatStamp 32 pos_infinity neg_infinity)"
+    by auto
+  have "join (FloatStamp 32 0 20) (FloatStamp 32 (-100) 10) = (FloatStamp 32 0 10)"
+    by auto
+  have "meet (FloatStamp 32 0 20) (FloatStamp 32 (-100) 10) = (FloatStamp 32 (- 100) 20)"
+    by auto
+end
 
 end
